# Logaritmus - Substituce

$\log^2x=(\log x)(\log x)=(\log x)^2$
$log(x^2)=2\log x$

$\log^2x+\log x^3+\log x^2=14$
$\log^2x+3\log x+2\log x=14$
$\log^2x+5\log x-14=0$

$a=\log x$
$a^2+5a-14=0$
$a_{1,2}=\frac{-b\pm\sqrt{b^2-4ac}}{2a}$
$a_{1,2}=\frac{-5\pm\sqrt{25-4*1*(-14)}}{2*1}$
$a_{1,2}=\frac{-5\pm\sqrt{81}}2=\frac{-5\pm9}2$
$a_1=2$
$a_2=-7$

$\log x=2$
$x=100$
$\log x = -7$

$x_1=100$
$x_2=10^{-7}$

$[x>0]$

$K=\{10^{-7};100\}$!



## Příklady


$\log^2x+\log x^2=0$
$(\log x)^2+2\log x=0$
$k=\log x$
$k^2+2k=0$

$k_{1,2}=\frac{-b\pm\sqrt{b^2-4ac}}{2a}$
$k_{1,2}=\frac{-2\pm\sqrt{2^2-4*1*0}}{2*1}$
$k_{1,2}=\frac{-2\pm2}{2}$
$k_1=-2$
$k_2=0$

$\log x=-2$

$\log x=0$

$x=10^{-2}=0.01$
$x=0$

---

$\log^2_3(x-1)-3\log_3(x-1)=10$
$(\log_3(x-1))^2-3\log_3(x-1)=10$
$k=\log_3(x-1)$
$k^2-3k-10=0$

$t^2-3t-10=0$
$(t+2)(t-5)=0$
$t_1=-2$
$t_2=5$
$\log_3(x-1)=t$
$\log_3(x-1)=-2$
$3^{-2}=x+1$
$1/9-1=x$
$x=8/9$
$\log_3(x-1)=5$
$3^5=x+1$
$243=x+1$
$x=242$

![](Pasted%20image%2020221219193816.png)

to pod tim neplati lmao xd
$k_{1,2}=\frac{-b\pm\sqrt{b^2-4ac}}{2a}$
$k_{1,2}=\frac{3\pm\sqrt{(-3)^2-4*1*10}}{2}$
$k_{1,2}=\frac{3\pm\sqrt{9-40}}2$
$k_{1,2}=\frac{3\pm}2$
$k_1=0$
$k_2=3$

$\log_3(x-1)=0$
$\log_3(x-1)=3$
$x=2$
$x=3$

---

$\log_2(\log_3(x+4))=1$

$\log_3(x+4)=2^1$
($2$ z $\log_2$, $1$ z strany za =)

$\log_3(x+4)=2$
$x+4=3^2$
$x+4=9$
$x=9-4$
$x=5$

---

